Locally Nameless STLC: Plenty of work on bidirectional typing.

LocallyNameless/STLC/Constants/Confluence.v
@@ -374,199 +374,6 @@ Qed.
 
 #[export] Hint Resolve ParallelStep_FullStep MultiStep_ParallelStep : core.
 
-Module development_try1.
-
-Fixpoint development (t : Tm) : Tm :=
-match t with
-| fvar x          => fvar x
-| bvar i          => bvar i
-| abs t'          => abs (development t' {{ 0 ~> fresh (fv t') }})
-| app (abs t1) t2 => development t1 {[ 0 ~> development t2 ]}
-| app t1 t2       => app (development t1) (development t2)
-| _               => unit
-end.
-
-Lemma development_open :
-  forall (t : Tm) (i : nat) (a : Atom),
-    lc t ->
-    development t {{ i ~> a }} = development (t {{ i ~> a }}).
-Proof.
-  intros.
-  rewrite (open_lc t i a) by easy.
-Abort.
-
-Lemma lc_development :
-  forall (t : Tm),
-    lc t -> lc (development t).
-Proof.
-  induction 1; cbn; auto.
-  - admit.
-Abort.
-
-End development_try1.
-
-Module development_try2.
-
-Unset Guard Checking.
-Fixpoint development (t : Tm) : Tm :=
-match t with
-| fvar x          => fvar x
-| bvar i          => bvar i
-| abs t'          => abs (development t')
-| app (abs t1) t2 =>
-  let x := fresh (fv t1) in
-    development (t1 {{ 0 ~> x }}) [[ x := development t2 ]]
-| app t1 t2       => app (development t1) (development t2)
-| _               => unit
-end.
-Set Guard Checking.
-
-Lemma development_open :
-  forall (t : Tm) (i : nat) (a : Atom),
-    development t {{ i ~> a }} = development (t {{ i ~> a }}).
-Proof.
-  induction t; cbn; intros; try now auto.
-  - now rewrite IHt.
-  - destruct t1; cbn in *; rewrite 1?IHt1, 1?IHt2; auto.
-    +
-Admitted.
-
-Lemma lc_development :
-  forall (t : Tm),
-    lc t -> lc (development t).
-Proof.
-  induction 1; cbn; auto.
-  - constructor 2 with l; intros x Hx.
-Admitted.
-
-Lemma development_spec :
-  forall t1 t2 : Tm,
-    ParallelStep t1 t2 -> ParallelStep t2 (development t1).
-Proof.
-  intros t1 t2 Hps.
-  assert (lc t2) by eauto.
-  induction Hps; cbn.
-  - now eauto.
-  - apply ParallelStep_abs with l; intros x Hx.
-    now rewrite development_open; eauto.
-  - destruct t1; cbn in *; try now auto.
-    inversion H; subst.
-Admitted.
-
-End development_try2.
-
-Module development_try3.
-
-Unset Guard Checking.
-Fixpoint development (t : Tm) : Tm :=
-match t with
-| fvar x          => fvar x
-| bvar i          => bvar i
-| abs t'          => abs (development t')
-| app (abs t1) t2 =>
-  let x := fresh (fv t1) in
-    development t1 {[ 0 ~> development t2 ]}
-| app t1 t2       => app (development t1) (development t2)
-| _               => unit
-end.
-Set Guard Checking.
-
-Lemma development_open :
-  forall (t : Tm) (i : nat) (a : Atom),
-    development t {{ i ~> a }} = development (t {{ i ~> a }}).
-Proof.
-  induction t; cbn; intros; auto.
-  - now rewrite IHt.
-  - destruct t1; cbn in *; rewrite 1?IHt1, 1?IHt2; auto.
-    + injection (IHt1 i a) as [= <-].
-      rewrite <- IHt2.
-Admitted.
-
-Lemma development_spec :
-  forall t1 t2 : Tm,
-    ParallelStep t1 t2 -> ParallelStep t2 (development t1).
-Proof.
-  induction 1; cbn.
-  - now eauto.
-  - apply ParallelStep_abs with l; intros x Hx.
-    now rewrite development_open; auto.
-  - destruct t1; cbn in *; try now auto.
-    inversion H; subst.
-    inversion IHParallelStep1; subst; eauto.
-  - 
-Admitted.
-
-End development_try3.
-
-Module development_try4.
-
-Fixpoint development (i : nat) (t : Tm) : Tm :=
-match t with
-| fvar x          => fvar x
-| bvar j          => bvar j
-| abs t'          => abs (development (S i) t')
-| app (abs t1) t2 => development (S i) t1 {[ 0 ~> development i t2 ]}
-| app t1 t2       => app (development i t1) (development i t2)
-| _               => unit
-end.
-
-End development_try4.
-
-Module development_try5.
-
-Unset Guard Checking.
-Fixpoint development (t : Tm) : Tm :=
-match t with
-| fvar x          => fvar x
-| bvar i          => bvar i
-| abs t'          =>
-  let x := fresh (fv t') in
-    abs (development (t' {{ 0 ~> x }}) {{ 0 <~ x }})
-| app (abs t1) t2 =>
-  let x := fresh (fv t1) in
-    development (t1 {{ 0 ~> x }}) [[ x := development t2 ]]
-| app t1 t2       => app (development t1) (development t2)
-| _               => unit
-end.
-Set Guard Checking.
-
-Lemma development_open :
-  forall (t : Tm) (i : nat) (a : Atom),
-    development t {{ i ~> a }} = development (t {{ i ~> a }}).
-Proof.
-  induction t; cbn; intros i x; try now auto.
-  - admit.
-  - destruct t1; cbn in *; rewrite 1?IHt1, 1?IHt2; auto.
-    + 
-Admitted.
-
-Lemma development_spec :
-  forall t1 t2 : Tm,
-    ParallelStep t1 t2 -> ParallelStep t2 (development t1).
-Proof.
-  induction 1; cbn.
-  - now eauto.
-  - apply ParallelStep_abs with l; intros x Hx.
-    apply ParallelStep_rename with (fresh (fv t1 ++ fv t2)).
-Admitted.
-
-End development_try5.
-
-Axiom development : Tm -> Tm.
-
-Axiom development_spec :
-  forall t1 t2 : Tm,
-    ParallelStep t1 t2 -> ParallelStep t2 (development t1).
-
-Lemma confluent_ParallelStep :
-  forall t t1 t2 : Tm,
-    ParallelStep t t1 -> ParallelStep t t2 ->
-      ParallelStep t1 (development t) /\ ParallelStep t2 (development t).
-Proof.
-  intros t t1 t2 Hps1 Hps2.
-  now split; apply development_spec.
-Qed.
-
 Inductive ParallelMultiStep : Tm -> Tm -> Prop :=
 | ParallelMultiStep_refl :
   forall (t : Tm),
@@ -655,6 +462,21 @@ Proof.
     now transitivity t2; eauto.
 Qed.
 
+Axiom development : Tm -> Tm.
+
+Axiom development_spec :
+  forall t1 t2 : Tm,
+    ParallelStep t1 t2 -> ParallelStep t2 (development t1).
+
+Lemma confluent_ParallelStep :
+  forall t t1 t2 : Tm,
+    ParallelStep t t1 -> ParallelStep t t2 ->
+      ParallelStep t1 (development t) /\ ParallelStep t2 (development t).
+Proof.
+  intros t t1 t2 Hps1 Hps2.
+  now split; apply development_spec.
+Qed.
+
 Lemma confluent_ParallelStep_ParallelMultiStep :
   forall t t1 t2 : Tm,
     ParallelStep t t1 -> ParallelMultiStep t t2 ->
@@ -691,106 +513,9 @@ Proof.
   now apply confluent_ParallelMultiStep.
 Qed.
 
-Inductive Development : Tm -> Tm -> Prop :=
-| Development_fvar :
-  forall (x : Atom),
-    Development x x
-| Development_abs :
-  forall (t1 t2 : Tm) (l : list Atom)
-    (Hps' : forall x : Atom, x # l -> Development (t1 {{ 0 ~> x }}) (t2 {{ 0 ~> x }})),
-    Development (abs t1) (abs t2)
-| Development_app :
-  forall (t1 t1' t2 t2' : Tm),
-    (forall u, t1 <> abs u) ->
-    Development t1 t1' ->
-    Development t2 t2' ->
-    Development (app t1 t2) (app t1' t2')
-| Development_app_abs :
-  forall (t1 t1' t2 t2' : Tm) (l : list Atom)
-    (Hps1 : forall x : Atom, x # l -> Development (t1 {{ 0 ~> x }}) (t1' {{ 0 ~> x }}))
-    (Hps2 : Development t2 t2'),
-    Development (app (abs t1) t2) (t1' {[ 0 ~> t2' ]}).
+Print Assumptions confluent_Step.
+Print Assumptions ParallelStep_refl.
+Print Assumptions MultiStep_abs.
+Print Assumptions confluent_Step.
 
-#[export] Hint Constructors Development : core.
 
-Lemma lc_Development_l :
-  forall t t' : Tm,
-    Development t t' -> lc t.
-Proof.
-  now induction 1; eauto.
-Qed.
-
-Lemma lc_Development_r :
-  forall t t' : Tm,
-    Development t t' -> lc t'.
-Proof.
-  now induction 1; eauto.
-Qed.
-
-#[export] Hint Resolve lc_Development_l lc_Development_r : core.
-
-Lemma Development_det :
-  forall t t1 t2 : Tm,
-    Development t t1 -> Development t t2 -> t1 = t2.
-Proof.
-  intros t t1 t2 Hd1 Hd2; revert t2 Hd2.
-  induction Hd1; inversion 1; subst.
-  - easy.
-  - now apply abs_eq with (fresh (l ++ l0 ++ fv t2 ++ fv t4)); auto.
-  - now erewrite IHHd1_1, IHHd1_2; eauto.
-  - now contradiction (H t3).
-  - now contradiction (H2 t1).
-  - rewrite !(open'_spec _ 0 (fresh (l ++ l0 ++ fv t1' ++ fv t1'0))) by auto.
-    now f_equal; auto.
-Qed.
-
-Lemma Development_FullContraction :
-  forall t1 t2 t3 : Tm,
-    FullContraction t1 t2 -> Development t2 t3 -> Development t1 t3.
-Proof.
-  do 2 inversion 1; subst.
-  - rewrite H4.
-    constructor 4 with l.
-Restart.
-  intros t1 t2 t3 H12 H23; revert t1 H12.
-  induction H23; intros.
-  - admit.
-  - inversion H12; subst.
-Admitted.
-
-Lemma FullStep_Development :
-  forall t1 t2 t3 : Tm,
-    FullStep t1 t2 -> Development t2 t3 -> Development t1 t3.
-Proof.
-  intros t1 t2 t3 Hfs Hd; revert t3 Hd.
-  induction Hfs; intros.
-  - now eapply Development_FullContraction; eauto.
-  - inversion Hd; subst.
-    constructor 2 with (l ++ l0); intros x Hx.
-    now eapply H; auto.
-  - inversion Hd; subst.
-    + constructor; [| now auto..].
-      intros u [= ->].
-      inversion Hfs; subst; [now inversion H0 |].
-      now contradiction (H2 t').
-    + inversion Hd; subst.
-      * now contradiction (H3 t0).
-      * 
-Restart.
-  intros t1 t2 t3 Hfs Hd; revert t1 Hfs.
-  induction Hd; intros.
-  - inversion Hfs; inversion H; subst.
-    destruct t0; cbn in H4; inversion H4; subst; cbn.
-Abort.
-
-Lemma MultiStep_Development :
-  forall t1 t2 : Tm,
-    Development t1 t2 -> MultiStep t1 t2.
-Proof.
-  induction 1; eauto.
-  transitivity (app (abs t1') t2); [now eapply MultiStep_app; eauto |].
-  transitivity (app (abs t1') t2'); [now eapply MultiStep_app; eauto |].
-  now apply MultiStep_FullStep; constructor; eauto.
-Qed.
-
-#[export] Hint Resolve MultiStep_Development : core.
