LocallyNameless/STLC/Constants/Dev1.v
@@ -1,0 +1,28 @@
+From FormalSystems Require Export LocallyNameless.STLC.Constants.Confluence.
+
+Fixpoint development (t : Tm) : Tm :=
+match t with
+| fvar x          => fvar x
+| bvar i          => bvar i
+| abs t'          => abs (development t' {{ 0 ~> fresh (fv t') }})
+| app (abs t1) t2 => development t1 {[ 0 ~> development t2 ]}
+| app t1 t2       => app (development t1) (development t2)
+| _               => unit
+end.
+
+Lemma development_open :
+  forall (t : Tm) (i : nat) (a : Atom),
+    lc t ->
+    development t {{ i ~> a }} = development (t {{ i ~> a }}).
+Proof.
+  intros.
+  rewrite (open_lc t i a) by easy.
+Abort.
+
+Lemma lc_development :
+  forall (t : Tm),
+    lc t -> lc (development t).
+Proof.
+  induction 1; cbn; auto.
+  - admit.
+Abort.
