LocallyNameless/STLC/Constants/Dev2.v
@@ -1,0 +1,47 @@
+From FormalSystems Require Export LocallyNameless.STLC.Constants.Confluence.
+
+Unset Guard Checking.
+Fixpoint development (t : Tm) : Tm :=
+match t with
+| fvar x          => fvar x
+| bvar i          => bvar i
+| abs t'          => abs (development t')
+| app (abs t1) t2 =>
+  let x := fresh (fv t1) in
+    development (t1 {{ 0 ~> x }}) [[ x := development t2 ]]
+| app t1 t2       => app (development t1) (development t2)
+| _               => unit
+end.
+Set Guard Checking.
+
+Lemma development_open :
+  forall (t : Tm) (i : nat) (a : Atom),
+    development t {{ i ~> a }} = development (t {{ i ~> a }}).
+Proof.
+  induction t; cbn; intros; try now auto.
+  - now rewrite IHt.
+  - destruct t1; cbn in *; rewrite 1?IHt1, 1?IHt2; auto.
+    +
+Admitted.
+
+Lemma lc_development :
+  forall (t : Tm),
+    lc t -> lc (development t).
+Proof.
+  induction 1; cbn; auto.
+  - constructor 2 with l; intros x Hx.
+Admitted.
+
+Lemma development_spec :
+  forall t1 t2 : Tm,
+    ParallelStep t1 t2 -> ParallelStep t2 (development t1).
+Proof.
+  intros t1 t2 Hps.
+  assert (lc t2) by eauto.
+  induction Hps; cbn.
+  - now eauto.
+  - apply ParallelStep_abs with l; intros x Hx.
+    now rewrite development_open; eauto.
+  - destruct t1; cbn in *; try now auto.
+    inversion H; subst.
+Admitted.
