LocallyNameless/STLC/Constants/Dev5.v
@@ -1,0 +1,105 @@
+From FormalSystems Require Export LocallyNameless.STLC.Constants.Confluence.
+
+Inductive Development : Tm -> Tm -> Prop :=
+| Development_fvar :
+  forall (x : Atom),
+    Development x x
+| Development_abs :
+  forall (t1 t2 : Tm) (l : list Atom)
+    (Hps' : forall x : Atom, x # l -> Development (t1 {{ 0 ~> x }}) (t2 {{ 0 ~> x }})),
+    Development (abs t1) (abs t2)
+| Development_app :
+  forall (t1 t1' t2 t2' : Tm),
+    (forall u, t1 <> abs u) ->
+    Development t1 t1' ->
+    Development t2 t2' ->
+    Development (app t1 t2) (app t1' t2')
+| Development_app_abs :
+  forall (t1 t1' t2 t2' : Tm) (l : list Atom)
+    (Hps1 : forall x : Atom, x # l -> Development (t1 {{ 0 ~> x }}) (t1' {{ 0 ~> x }}))
+    (Hps2 : Development t2 t2'),
+    Development (app (abs t1) t2) (t1' {[ 0 ~> t2' ]}).
+
+#[export] Hint Constructors Development : core.
+
+Lemma lc_Development_l :
+  forall t t' : Tm,
+    Development t t' -> lc t.
+Proof.
+  now induction 1; eauto.
+Qed.
+
+Lemma lc_Development_r :
+  forall t t' : Tm,
+    Development t t' -> lc t'.
+Proof.
+  now induction 1; eauto.
+Qed.
+
+#[export] Hint Resolve lc_Development_l lc_Development_r : core.
+
+Lemma Development_det :
+  forall t t1 t2 : Tm,
+    Development t t1 -> Development t t2 -> t1 = t2.
+Proof.
+  intros t t1 t2 Hd1 Hd2; revert t2 Hd2.
+  induction Hd1; inversion 1; subst.
+  - easy.
+  - now apply abs_eq with (fresh (l ++ l0 ++ fv t2 ++ fv t4)); auto.
+  - now erewrite IHHd1_1, IHHd1_2; eauto.
+  - now contradiction (H t3).
+  - now contradiction (H2 t1).
+  - rewrite !(open'_spec _ 0 (fresh (l ++ l0 ++ fv t1' ++ fv t1'0))) by auto.
+    now f_equal; auto.
+Qed.
+
+Lemma Development_FullContraction :
+  forall t1 t2 t3 : Tm,
+    FullContraction t1 t2 -> Development t2 t3 -> Development t1 t3.
+Proof.
+  do 2 inversion 1; subst.
+  - rewrite H4.
+    constructor 4 with l.
+Restart.
+  intros t1 t2 t3 H12 H23; revert t1 H12.
+  induction H23; intros.
+  - admit.
+  - inversion H12; subst.
+Admitted.
+
+Lemma FullStep_Development :
+  forall t1 t2 t3 : Tm,
+    FullStep t1 t2 -> Development t2 t3 -> Development t1 t3.
+Proof.
+  intros t1 t2 t3 Hfs Hd; revert t3 Hd.
+  induction Hfs; intros.
+  - now eapply Development_FullContraction; eauto.
+  - inversion Hd; subst.
+    constructor 2 with (l ++ l0); intros x Hx.
+    now eapply H; auto.
+  - inversion Hd; subst.
+    + constructor; [| now auto..].
+      intros u [= ->].
+      inversion Hfs; subst; [now inversion H0 |].
+      now contradiction (H2 t').
+    + inversion Hd; subst.
+      * now contradiction (H3 t0).
+      * 
+Restart.
+  intros t1 t2 t3 Hfs Hd; revert t1 Hfs.
+  induction Hd; intros.
+  - inversion Hfs; inversion H; subst.
+    destruct t0; cbn in H4; inversion H4; subst; cbn.
+Abort.
+
+Lemma MultiStep_Development :
+  forall t1 t2 : Tm,
+    Development t1 t2 -> MultiStep t1 t2.
+Proof.
+  induction 1; eauto.
+  transitivity (app (abs t1') t2); [now eapply MultiStep_app; eauto |].
+  transitivity (app (abs t1') t2'); [now eapply MultiStep_app; eauto |].
+  now apply MultiStep_FullStep; constructor; eauto.
+Qed.
+
+#[export] Hint Resolve MultiStep_Development : core.
